dia 10

src/Knapsack/Implementation/Input.dfy
@@ -20,15 +20,47 @@ class Input {
     items[i].Model()
   }
 
-  ghost function Model() : InputData
+
+
+  /*ghost function Model() : InputData
     reads this, items, set i | 0 <= i < items.Length :: items[i]
   {
     InputData(seq(items.Length, ModelAt), maxWeight)
+  }*/
+
+
+  ghost function ItemsUntil(k: nat): seq<ItemData>
+    reads this, items, set i | 0 <= i < k :: items[i]
+    requires k <= items.Length
+    ensures |ItemsUntil(k)| == k
+    ensures forall i | 0 <= i < k :: ItemsUntil(k)[i].weight == items[i].weight
+    ensures forall i | 0 <= i < k :: ItemsUntil(k)[i].value == items[i].value
+  {
+    if k == 0 then
+      []
+    else
+      ItemsUntil(k-1) + [items[k-1].Model()]
   }
+
+  ghost function Model() : InputData
+    reads this, items, set i | 0 <= i < items.Length :: items[i]
+    ensures |Model().items| == items.Length
+    ensures forall i | 0 <= i < items.Length :: Model().items[i].weight == items[i].weight
+    ensures forall i | 0 <= i < items.Length :: Model().items[i].value == items[i].value
+  {
+    InputData(ItemsUntil(items.Length), maxWeight)
+  }
+
 
   ghost predicate Valid()
     reads this, items, set i | 0 <= i < items.Length :: items[i] //añadido esto ultimo, era necesario también
   {
     this.Model().Valid()
   }
+
+   lemma InputDataItems(k:int)
+  requires 0 <= k < items.Length
+  ensures items[k].weight == Model().items[k].weight
+  ensures items[k].value == Model().items[k].value
+  {}
 }
